theories/base.v
@@ -1,3 +1,5 @@
+From Ltac2 Require Export Ltac2 Rewrite.
+
 (** Global notation declarations. *)
 Declare Scope stlc_scope.
 Delimit Scope stlc_scope with stlc.
