theories/tactics.v
@@ -1,0 +1,103 @@
+From Stdlib Require Import Lia.
+Require Export base.
+
+
+Ltac2 rec c_injection l h :=
+  let h1 := Fresh.in_goal @IA in let h2 := Fresh.in_goal @IB in
+  apply $l in $h as [$h1 $h2];
+  let f x := Control.plus (fun () => c_injection l x) (
+    fun _ => let c := Control.hyp x in try (rewrite $c in *); clear $x
+  ) in
+  f h1; f h2.
+(*
+  let c1 := Control.hyp h1 in let c2 := Control.hyp h2 in
+  try (rewrite $c1 in * ); try (rewrite $c2 in * ).
+  *)
+
+
+Ltac2 s_simpl c := Std.simpl {
+    Std.rStrength := Std.Norm;
+    Std.rBeta := true;
+    Std.rMatch := true;
+    Std.rFix := true;
+    Std.rCofix := true;
+    Std.rZeta := true;
+    Std.rDelta := true;
+    Std.rConst := []
+  }
+  None
+  c
+  .
+
+Ltac2 all_hyps t :=
+  List.iter (
+    fun (x, _, _) => t x
+  ) (Control.hyps ()).
+
+Ltac2 autorewrite (dt : ident) (c : Std.clause) :=
+  match c.(Std.on_hyps) with
+  | None => all_hyps (fun x => ltac1:(dt x |- autorewrite with dt in x) (Ltac1.of_ident dt) (Ltac1.of_ident x))
+  | Some l => List.iter (fun (x, _, _) => ltac1:(dt x |- autorewrite with dt in x) (Ltac1.of_ident dt) (Ltac1.of_ident x)) l
+  end;
+  match c.(Std.on_concl) with
+  | Std.AllOccurrences => ltac1:(dt |- autorewrite with dt) (Ltac1.of_ident dt)
+  | _ => ()
+  end.
+
+Ltac2 Notation "easy" := ltac1:(easy).
+Ltac2 Notation easy := easy.
+Ltac2 Notation "lia" := ltac1:(lia).
+Ltac2 Notation lia := lia.
+Ltac2 Notation "intuition" := ltac1:(intuition).
+
+Ltac2 goal := {
+    Std.on_hyps := Some [];
+    Std.on_concl := Std.AllOccurrences
+  }.
+Ltac2 one_hyp h := {
+    Std.on_hyps := Some [(h, Std.AllOccurrences, Std.InHyp)];
+    Std.on_concl := Std.NoOccurrences
+  }.
+Ltac2 all := {
+    Std.on_hyps := None;
+    Std.on_concl := Std.AllOccurrences
+  }.
+
+
+Ltac2 Type view_parameters := {
+  to_tp : constr;
+  to_view : constr;
+  to_tp_to_view : constr;
+  tp_simpl : Std.clause -> unit;
+  discriminate_other : constr -> unit
+}.
+
+Ltac2 to_tp p h :=
+  let to_tp := p.(to_tp) in let to_tp_to_view := p.(to_tp_to_view) in
+  apply (f_equal $to_tp) in $h; repeat (rewrite $to_tp_to_view in $h).
+
+Ltac2 to_view p (h : ident) :=
+  let to_view := p.(to_view) in
+  apply (f_equal $to_view) in $h; p.(tp_simpl) (one_hyp h).
+
+Ltac2 tp_injection p (h : ident) :=
+  to_view p h;
+  let c := Control.hyp h in
+  let no := List.length (Control.hyps ()) in
+  Std.move h Std.MoveLast; injection $c as ?;
+  List.iter (
+    fun (x, _, _) => try (to_tp p x);
+    let cx := Control.hyp x in rewrite $cx in *; clear $x
+  ) (List.skipn (Int.sub no 1) (Control.hyps ())).
+
+Ltac2 tp_discriminate p (h : ident) :=
+  let c := Control.hyp h in
+  lazy_match! (Constr.type c) with
+  | _ = _ => to_view p h; discriminate $c
+  | _ => p.(discriminate_other) c
+  end.
+
+Ltac2 tp_discriminate_all p :=
+  match! goal with
+  | [h : _ |- _] => tp_discriminate p h
+  end.
